theories/c_toy_mlang/class_instances.v
@@ -1,0 +1,158 @@
+From melocoton.language Require Import mlanguage.
+From melocoton.c_toy_mlang Require Export lang.
+From melocoton.c_toy_mlang Require Import tactics notation.
+From melocoton.c_toy_mlang Require Import lang_instantiation.
+From iris.prelude Require Import options.
+
+Global Instance into_val_val v : @IntoVal C_mlang_melocoton (Val v) v.
+Proof. done. Qed.
+Global Instance as_val_val v : @AsVal C_mlang_melocoton (Val v).
+Proof. by eexists. Qed.
+
+Lemma clang_sub_redexes_are_values e :
+  (∀ Ki e', e = fill_item Ki e' → is_Some (mlanguage.to_val e')) →
+  sub_redexes_are_values e.
+Proof.
+  intros Hsub K e' ->. destruct K as [|Ki K _] using @rev_ind=> //=.
+  intros []%eq_None_not_Some.
+  eapply mlanguage.fill_val, Hsub. by rewrite /= fill_app.
+Qed.
+
+(** * Instances of the [Atomic] class *)
+Section atomic.
+  Context {p:program}.
+
+  Local Ltac solve_atomic :=
+    apply mlanguage_atomic;
+      [intros H1 H2 H3 Hstep; inversion Hstep; try naive_solver; congruence
+      |apply clang_sub_redexes_are_values; intros [] **; naive_solver].
+
+  (** The instance below is a more general version of [Skip] *)
+  Global Instance let_atomic x v1 v2 : Atomic (Let x (Val v1) (Val v2)).
+  Proof.
+    apply mlanguage_atomic.
+    { intros ? ? ? Hstep. inversion Hstep; subst.
+
+      [intros H1 H2 H3 Hstep; inversion Hstep; try naive_solver; congruence
+      |apply clang_sub_redexes_are_values; intros [] **; naive_solver].
+
+
+    destruct x; solve_atomic. Qed.
+  Global Instance unop_atomic op v : Atomic (UnOp op (Val v)).
+  Proof. solve_atomic. Qed.
+  Global Instance binop_atomic op v1 v2 : Atomic (BinOp op (Val v1) (Val v2)).
+  Proof. solve_atomic. Qed.
+  Global Instance if_true_atomic v v1 e2 : asTruth v = true ->
+    Atomic (If (Val $ v) (Val v1) e2).
+  Proof. intros H. solve_atomic. Qed.
+  Global Instance if_non_zero_atomic (v0:Z) v1 e2 : v0 ≠ 0%Z ->
+    Atomic (If (Val $ LitV $ LitInt v0) (Val v1) e2).
+  Proof. intros H. apply if_true_atomic. destruct v0; cbn; congruence. Qed.
+  Global Instance if_true_bool_atomic v1 e2 :
+    Atomic (If (Val $ LitV $ LitBool true) (Val v1) e2).
+  Proof. intros H. apply if_true_atomic. easy. Qed.
+  Global Instance if_false_atomic v e1 v2 : asTruth v = false ->
+    Atomic (If (Val $ v) e1 (Val v2)).
+  Proof. intros H. solve_atomic. Qed.
+  Global Instance if_zero_atomic e1 v2 :
+    Atomic (If (Val $ LitV $ LitInt (0%Z)) e1 (Val v2)).
+  Proof. intros H. apply if_false_atomic. easy. Qed.
+  Global Instance if_false_bool_atomic e1 v2 :
+    Atomic (If (Val $ LitV $ LitBool false) e1 (Val v2)).
+  Proof. intros H. apply if_false_atomic. easy. Qed.
+
+  Global Instance alloc_atomic v : Atomic (Malloc (Val v)).
+  Proof. solve_atomic. Qed.
+  Global Instance free_atomic v1 v2 : Atomic (Free (Val v1) (Val v2)).
+  Proof. solve_atomic. Qed.
+  Global Instance load_atomic v : Atomic (Load (Val v)).
+  Proof. solve_atomic. Qed.
+  Global Instance store_atomic v1 v2 : Atomic (Store (Val v1) (Val v2)).
+  Proof. solve_atomic. Qed.
+
+End atomic.
+
+Section pure_exec.
+  Context {p:program}.
+  (* Local Ltac solve_exec_safe := intros; subst; do 4 eexists; try (econstructor; eauto; done). *)
+  (* Local Ltac solve_exec_puredet := simpl; intros; inv_head_step; try done. *)
+  (* Local Ltac solve_pure_exec := *)
+  (*   subst; intros ?; apply nsteps_once, pure_head_step_pure_step; *)
+  (*     constructor; [solve_exec_safe | solve_exec_puredet]. *)
+
+  Local Ltac solve_exec_safe :=
+    intros; subst; try (exists (λ _, True); econstructor; eauto; done).
+  Local Ltac solve_exec_puredet :=
+    intros; cbn; try (econstructor; by eauto).
+  Local Ltac solve_pure_exec :=
+    subst; intros ?; apply multirelations.repeat_once, pure_head_step_pure_step;
+      constructor; [solve_exec_safe | solve_exec_puredet].
+
+  Local Ltac destruct_bool_decide := repeat (let H := fresh "Heq" in
+    try destruct bool_decide eqn:H;
+    [apply bool_decide_eq_true_1 in H| apply bool_decide_eq_false_1 in H]).
+
+  Global Instance pure_let x (v1 v2 : val) :
+    PureExec True 1 p (Let x (Val v1) (Val v2)) (singl (subst' x v1 v2)).
+  Proof. solve_pure_exec. Qed.
+
+  Global Instance pure_unop op v v' :
+    PureExec (un_op_eval op v = Some v') 1 p (UnOp op (Val v)) (singl (Val v')).
+  Proof. solve_pure_exec. Qed.
+
+  Global Instance pure_binop op v1 v2 v' :
+    PureExec (bin_op_eval op v1 v2 = Some v') 1 p (BinOp op (Val v1) (Val v2)) (singl (Val (LitV v'))) | 10.
+  Proof. solve_pure_exec. Qed.
+
+  (* Higher-priority instance for [EqOp]. *)
+  Global Instance pure_eqop v1 v2 :
+    PureExec (vals_compare_safe v1 v2) 1 p
+      (BinOp EqOp (Val (LitV v1)) (Val (LitV v2)))
+      (singl (Val $ LitV $ LitBool $ bool_decide (v1 = v2))) | 1.
+  Proof.
+    intros Hcompare.
+    cut (bin_op_eval EqOp (LitV v1) (LitV v2) = Some $ LitBool $ bool_decide (v1 = v2)).
+    { intros. revert Hcompare. solve_pure_exec. }
+    destruct v1, v2; cbn in *; try easy.
+    - destruct_bool_decide; congruence.
+    - destruct l, l0. destruct_bool_decide; congruence.
+    - destruct_bool_decide; congruence.
+  Qed.
+
+  Global Instance pure_if_true v e1 e2 : asTruth v = true ->
+    PureExec True 1 p (If (Val $ v) e1 e2) (singl e1).
+  Proof. intros H. solve_pure_exec. Qed.
+  Global Instance pure_if_non_zero (v0:Z) e1 e2 : v0 ≠ 0%Z ->
+    PureExec True 1 p (If (Val $ LitV $ LitInt v0) e1 e2) (singl e1).
+  Proof. intros H. apply pure_if_true. destruct v0; cbn; congruence. Qed.
+  Global Instance pure_if_true_bool e1 e2 :
+    PureExec True 1 p (If (Val $ LitV $ LitBool true) e1 e2) (singl e1).
+  Proof. apply pure_if_true. easy. Qed.
+  Global Instance pure_if_false v e1 e2 : asTruth v = false ->
+    PureExec True 1 p (If (Val $ v) e1 e2) (singl e2).
+  Proof. intros H. solve_pure_exec. Qed.
+  Global Instance pure_if_zero e1 e2 :
+    PureExec True 1 p (If (Val $ LitV $ LitInt (0%Z)) e1 e2) (singl e2).
+  Proof. apply pure_if_false. easy. Qed.
+  Global Instance pure_if_false_bool e1 e2 :
+    PureExec True 1 p (If (Val $ LitV $ LitBool false) e1 e2) (singl e2).
+  Proof. apply pure_if_zero. Qed.
+
+  Global Instance pure_while e1 e2 :
+    PureExec True 1 p (While e1 e2) (singl (If e1 (Let BAnon e1 (While e1 e2)) (Val $ LitV $ LitInt 0))).
+  Proof. solve_pure_exec. Qed.
+
+  Global Instance pure_funcall s va args res e :
+    PureExec ((p : gmap.gmap string function) !! s = Some (Fun args e) ∧ zip_args args va = Some res) 1 p
+             (FunCall (Val $ LitV $ LitFunPtr s) (map Val va))
+             (singl (subst_all res e)).
+  Proof.
+    solve_pure_exec; destruct H as [H1 H2].
+    { exists (λ _, True). econstructor; eauto.
+      rewrite /apply_function H2//. }
+    { econstructor; eauto.
+      - rewrite /apply_function H2//.
+      - rewrite /singl //. }
+  Qed.
+
+End pure_exec.
